Refactored LTL lemmas and definitions into LTL file

fairneris/examples/retransmit_model_ltl.v
@@ -126,21 +126,8 @@ Proof. apply make_decision. Qed.
 
 Notation mtrace := (trace retransmit_state retransmit_label).
 
-Declare Scope trace_scope.
-Delimit Scope trace_scope with trace.
-Bind Scope trace_scope with trace.
-
-Notation "□ P" := (trace_always P) (at level 20, right associativity) : trace_scope.
-Notation "◊ P" := (trace_eventually P) (at level 20, right associativity) : trace_scope.
-Notation "↓ P" := (trace_now P) (at level 20, right associativity) : trace_scope.
-Notation "P → Q" := (trace_implies P Q)
-                      (at level 99, Q at level 200,
-                         format "'[' P  →  '/' '[' Q ']' ']'") : trace_scope.
-
 (* Definition retransmit_fair_network_delivery msg : mtrace → Prop := *)
 (*   □ (□◊↓send_filter msg → ◊↓deliver_filter msg). *)
-Definition trace_weak_until {S L} (P Q : trace S L → Prop) : trace S L → Prop :=
-  trace_or (trace_until P Q) (□ P).
 Definition retransmit_fair_network_delivery msg : mtrace → Prop :=
   □ ((trace_weak_until (□◊↓send_filter msg) (↓deliver_filter msg)) → ◊↓deliver_filter msg).
 
@@ -198,29 +185,6 @@ Definition trans_valid (mtr : mtrace) :=
 Definition mtrace_valid (mtr : mtrace) :=
   trace_always trans_valid mtr.
 
-Lemma trace_eventually_cons {S L} (P : trace S L → Prop) s l (tr : trace S L) :
-  trace_eventually P tr → trace_eventually P (s -[l]-> tr).
-Proof.
-  intros [n [Htr1 Htr2]].
-  exists (Datatypes.S n).
-  split; [done|]. clear Htr1.
-  intros m Hm.
-  destruct m; [by eexists _|].
-  apply Htr2. lia.
-Qed.
-
-Lemma trace_always_cons {S L} (P : trace S L → Prop) s l (tr : trace S L) :
-  trace_always P (s -[l]-> tr) → trace_always P tr.
-Proof.
-  rewrite /trace_always.
-  intros Htr Htr'. apply Htr. clear Htr.
-  by apply trace_eventually_cons.
-Qed.
-
-Lemma trace_always_now_cons {S L} (P : S → option L → Prop) s l (tr : trace S L) :
-  trace_always (trace_now P) (s -[l]-> tr) → P s (Some l).
-Proof. Admitted.
-
 Definition option_lift {S L} (P : S → L → Prop) : S → option L → Prop :=
   λ s ol, ∃ l, ol = Some l ∧ P s l.
 
@@ -228,186 +192,12 @@ Lemma option_lift_Some {S L} (P : S → L → Prop) s l :
   option_lift P s (Some l) → P s l.
 Proof. intros (l'&Hl'&HP). by simplify_eq. Qed.
 
-Lemma trace_eventually_mono {S L} (P Q : trace S L → Prop) tr :
-  (∀ tr, P tr → Q tr) → trace_eventually P tr → trace_eventually Q tr.
-Proof.
-  intros HPQ (n&(tr'&Htr1&Htr2)&H2).
-  exists n. split; [|done]. exists tr'. split; [done|]. by apply HPQ.
-Qed.
-
-Definition trace_suffix_of {S L} (tr1 tr2 : trace S L) : Prop :=
-  ∃ n, after n tr2 = Some tr1.
-
-Lemma trace_suffix_of_refl {S L} (tr : trace S L) :
-  trace_suffix_of tr tr.
-Proof. by exists 0. Qed.
-
-Lemma trace_eventually_mono_strong {S L} (P Q : trace S L → Prop) tr :
-  (∀ tr', trace_suffix_of tr' tr → P tr' → Q tr') →
-  trace_eventually P tr → trace_eventually Q tr.
-Proof.
-  intros HPQ (n&(tr'&Htr1&Htr2)&H2).
-  exists n. split; [|done]. exists tr'. split; [done|]. apply HPQ; [|done].
-  exists n. done.
-Qed.
-
-Lemma trace_implies_implies {S L} (P Q : trace S L → Prop) tr :
-  trace_implies P Q tr ↔ (P tr → Q tr).
-Proof.
-  split.
-  - by intros [|].
-  - intros HPQ.
-    assert (P tr ∨ ¬ P tr) as [HP|HP] by apply ExcludedMiddle.
-    + by right; apply HPQ.
-    + by left.
-Qed.
-
-Lemma trace_always_mono {S L} (P Q : trace S L → Prop) tr :
-  (∀ tr, trace_implies P Q tr) → trace_always P tr → trace_always Q tr.
-Proof.
-  intros HPQ HP HQ. apply HP. eapply trace_eventually_mono; [|done].
-  clear HP HQ. intros tr' HP HQ. apply HP.
-  specialize (HPQ tr'). rewrite trace_implies_implies in HPQ. by apply HPQ.
-Qed.
-
-Lemma trace_always_mono_strong {S L} (P Q : trace S L → Prop) tr :
-  (∀ tr', trace_suffix_of tr' tr → trace_implies P Q tr') → trace_always P tr → trace_always Q tr.
-Proof.
-  intros HPQ HP HQ. apply HP. eapply trace_eventually_mono_strong; [|done].
-  clear HP HQ. intros tr' Htr' HP HQ. apply HP.
-  specialize (HPQ tr'). rewrite trace_implies_implies in HPQ. by apply HPQ.  
-Qed.
-
-Lemma after_is_Some_lt {S L} (tr : trace S L) n m :
-  m < n → is_Some $ after n tr → is_Some $ after m tr.
-Proof.
-  revert tr m.
-  induction n; intros tr m Hle.
-  { intros. assert (m = 0) as -> by lia. done. }
-  intros.
-  destruct m; [done|].
-  simpl in *.
-  destruct tr; [done|].
-  apply IHn. lia. done.
-Qed.
-
-(* TODO: Improve this proof *)
-Lemma trace_alwaysI {S L} (P : trace S L → Prop) tr :
-  trace_always P tr ↔ (∀ tr', trace_suffix_of tr' tr → trace_always P tr').
-Proof.
-  split.
-  - rewrite /trace_always. 
-    intros Halways tr' [n Hafter] HP. apply Halways.
-    destruct HP as [m [HP HP']].
-    destruct HP as [tr'' [Htr'' Hnot]].
-    exists (n + m).
-    split.
-    + exists tr''. rewrite after_sum'. rewrite Hafter. done.
-    + intros m' Hlt.
-      assert (after (n+m) tr = Some tr'').
-      { rewrite after_sum'. rewrite Hafter. done. } 
-      assert (is_Some $ after m' tr) as [tr''' Htr'''].
-      { by eapply after_is_Some_lt. }
-      exists tr'''. split; [done|].
-      by destruct tr'''.
-  - intros Halways. eapply (Halways). apply trace_suffix_of_refl.
-Qed.
-
-Lemma trace_always_suffix_of {S L} (P : trace S L → Prop) tr1 tr2 :
-  trace_suffix_of tr2 tr1 → trace_always P tr1 → trace_always P tr2.
-Proof. rewrite (trace_alwaysI _ tr1). intros Hsuffix HP. by eapply HP. Qed.
-
-Lemma trace_always_universal {S L} (P : trace S L → Prop) (tr : trace S L) :
-  (∀ tr, P tr) → trace_always P tr.
-Proof. by intros ?(?&(?&_&?)&_); eauto. Qed.
-
 Lemma A_always_live (mtr : mtrace) :
   trace_always (trace_now (λ s _, retransmit_role_enabled_model (inl Arole) s)) mtr.
 Proof. apply trace_always_universal. 
   rewrite /pred_at /retransmit_role_enabled_model. intros mtr'.
   by destruct mtr'; set_solver.
 Qed.
-
-Lemma trace_not_idemp {S L} (P : trace S L → Prop) (tr : trace S L) :
-  trace_not (trace_not P) tr ↔ P tr.
-Proof. rewrite /trace_not. split; [apply NNP_P|apply P_NNP]. Qed.
-
-(* TODO: Replace existing lemma with this *)
-Lemma not_exists_forall_not_alt {A} (P : A → Prop) x : ¬ (∃ x, P x) → ¬ P x.
-Proof. intros Hnex HP; apply Hnex; eauto. Qed.
-
-Lemma trace_always_elim {S L} (P : trace S L → Prop) (tr : trace S L) :
-  trace_always P tr → P tr.
-Proof.
-  intros Htr.
-  eapply (not_exists_forall_not_alt _ 0) in Htr.
-  apply Classical_Prop.not_and_or in Htr as [Htr|Htr].
-  { eapply (not_exists_forall_not_alt _ tr) in Htr.
-    apply Classical_Prop.not_and_or in Htr as [Htr|Htr]; [done|].
-    apply trace_not_not in Htr. by rewrite trace_not_idemp in Htr. }
-  eapply not_forall_exists_not in Htr as [x Htr].
-  eapply Classical_Prop.imply_to_and in Htr as [Hx Htr].
-  lia.
-Qed.
-
-(* TODO: This is a bit of a weird statement *)
-Lemma trace_always_implies {S L} (P Q : trace S L → Prop) tr :
-  trace_always (trace_implies P Q) tr → trace_always P tr → trace_always Q tr.
-Proof.
-  intros HPQ HP.
-  eapply trace_always_mono_strong; [|done].
-  intros tr' Hsuffix.
-  apply trace_always_elim.
-  by eapply trace_always_suffix_of.
-Qed.
-
-Lemma trace_always_eventually_always_implies {S L} (P Q : trace S L → Prop) tr :
-  trace_always_eventually_implies P Q tr → trace_always P tr → trace_eventually Q tr.
-Proof.
-  intros HPQ HP.
-  eapply trace_always_implies in HP; [|done].
-  by apply trace_always_elim.
-Qed.  
-
-Lemma trace_always_eventually_always_mono {S L} (P1 P2 Q1 Q2 : trace S L → Prop) tr :
-  (∀ tr, trace_implies P2 P1 tr) → (∀ tr, trace_implies Q1 Q2 tr) →
-  trace_always_eventually_implies P1 Q1 tr → trace_always_eventually_implies P2 Q2 tr.
-Proof.
-  setoid_rewrite trace_implies_implies.
-  intros HP HQ Htr.
-  eapply trace_always_mono; [|done].
-  intros Htr'.
-  apply trace_implies_implies.
-  rewrite !trace_implies_implies.
-  intros HPQ HP2.
-  eapply trace_eventually_mono; [apply HQ|by apply HPQ; apply HP].
-Qed.
-
-Lemma trace_implies_refl {S L} (P : trace S L → Prop) tr :
-  trace_implies P P tr.
-Proof. by apply trace_implies_implies. Qed.
-
-(* This seems a bit too specific *)
-
-Definition trfirst_label {S L} (tr: trace S L) : option L :=
-  match tr with
-  | ⟨_⟩ => None
-  | _ -[ℓ]-> _ => Some ℓ
-  end.
-
-(* This seems a bit too specific *)
-Lemma trace_now_mono_strong {S L} (P Q : S → option L → Prop) tr :
-  (∀ s l, trfirst tr = s → trfirst_label tr = l → P s l → Q s l) →
-  trace_now P tr → trace_now Q tr.
-Proof.
-  destruct tr as [s|s l tr].
-  - rewrite /trace_now /pred_at /=. intros HPQ Htr. by apply HPQ.
-  - rewrite /trace_now /pred_at /=. intros HPQ Htr. by apply HPQ.
-Qed.
-
-Lemma trace_now_mono {S L} (P Q : S → option L → Prop) tr :
-  (∀ s l, P s l → Q s l) → trace_now P tr → trace_now Q tr.
-Proof. intros. eapply trace_now_mono_strong; [|done]. by eauto. Qed.
 
 Lemma retransmit_fair_traces_eventually_A mtr :
   retransmit_fair_scheduling_mtr (inl Arole) mtr →
@@ -442,31 +232,10 @@ Proof.
   simplify_eq. inversion Hvalid. inversion H1. by simplify_eq.
 Qed.
 
-Lemma trace_always_idemp {S L} P (tr : trace S L) :
-  (□ P) tr → (□ □ P) tr. 
-Proof. Admitted.
-
-Lemma trace_always_and {S L} P Q (tr : trace S L) :
-  ((□ P) tr ∧ (□ Q) tr) ↔ (□ trace_and P Q) tr. 
-Proof. Admitted.
-
 Lemma retransmit_fair_traces_always_eventually_mAB mtr :
   mtrace_valid mtr → retransmit_fair_scheduling_mtr (inl $ Arole) mtr →
   (□ ◊ ↓ send_filter mAB) mtr.
 Proof. Admitted.
-
-Lemma trace_or_l {S L} (P Q : trace S L → Prop) (tr : trace S L) :
-  P tr → trace_or P Q tr.
-Proof. intros HP. by left. Qed.
-
-Lemma trace_or_r {S L} (P Q : trace S L → Prop) (tr : trace S L) :
-  Q tr → trace_or P Q tr.
-Proof. intros HP. by right. Qed.
-
-Lemma trace_weak_until_always {S L} P Q (tr : trace S L) :
-  trace_always P tr → trace_weak_until P Q tr.
-Proof. intros HP. by apply trace_or_r. Qed.
-
 
 (* Any fair trace eventually delivers a message *)
 Lemma eventually_send_eventually_deliver mtr :
@@ -492,82 +261,6 @@ Qed.
 (*   apply H. apply trace_weak_until_always. apply trace_always_idemp. *)
 (*   by apply retransmit_fair_traces_always_eventually_mAB. *)
 (* Qed. *)
-
-Definition trace_next {S L} (P : trace S L → Prop) (tr : trace S L) : Prop :=
-  ∀ tr', after 1 tr  = Some tr' → P tr'.
-
-Notation "○ P" := (trace_next P) (at level 20, right associativity) : trace_scope.
-
-Lemma trace_eventually_next {S L} (P : trace S L → Prop) (tr : trace S L) :
-  (◊ ○ P) tr → (◊ P) tr.
-Proof.
-  (* destruct 1 as [n [HP HP']]. *)
-  (* destruct HP as [tr' [HP1 HP2]]. *)
-  (* destruct tr. *)
-  (* - admit. *)
-  (* - simpl in *. *)
-  (*   destruct n; simpl in *. *)
-  (*   + simplify_eq. exists 0.  split. *)
-  (*   + exists tr'. simpl in *. done. *)
-Admitted.
-
-Lemma trace_trueI {S L} (tr : trace S L) :
-  trace_true tr.
-Proof. destruct tr; done. Qed.
-
-Lemma trace_eventually_suffix_of {S L} (P : trace S L → Prop) tr1 tr2 :
-  trace_suffix_of tr1 tr2 → trace_eventually P tr1 → trace_eventually P tr2.
-Proof.
-  intros [n Hsuffix] [m [[tr' [Hafter HP]] Htrue]].
-  exists (n + m).
-  rewrite after_sum'. rewrite Hsuffix Hafter.
-  split.
-  - exists tr'. done.
-  - intros m' Hm.
-    assert (after (n + m) tr2 = Some tr').
-    { rewrite after_sum'. rewrite Hsuffix Hafter. done. }
-    assert (is_Some (after m' tr2)) as [tr'' Htr'].
-    { by eapply after_is_Some_lt. }
-    exists tr''. split; [done| apply trace_trueI].
-Qed.
-
-Lemma trace_eventually_thing_strong {S L} (P Q : trace S L → Prop) (tr : trace S L) :
-  (∀ tr', trace_suffix_of tr' tr → P tr' → (◊ Q) tr') → (◊ P) tr → (◊ Q) tr.
-Proof.
-  intros HPQ HP.
-  destruct HP as [n [[tr' [Hafter HP]] Htrue]].
-  apply HPQ in HP; [|by exists n].
-  eapply trace_eventually_suffix_of; [|done].
-  by exists n.
-Qed.
-
-Lemma trace_not_eventually_always_not {S L} P (tr : trace S L) :
-  trace_not (◊ P) tr ↔ (□ (trace_not P)) tr.
-Proof. Admitted.
-
-Lemma trace_always_eventually {S L} P (tr : trace S L) :
-  (□ P) tr → (◊ P) tr.
-Proof. Admitted.
-
-Lemma trace_not_now {S L} P (tr : trace S L) :
-  trace_not (↓ P) tr ↔ (↓ (λ s l, ¬ P s l)) tr.
-Proof. Admitted.
-
-Lemma trace_eventually_now {S L} P (tr : trace S L) :
-  (↓ P) tr → (◊ ↓ P) tr.
-Proof. Admitted.
-
-Lemma trace_now_exists {A} {S L} (P : A → S → option L → Prop) (tr : trace S L) :
-  (↓ (λ s l, ∃ (x:A), P x s l)) tr → ∃ (x:A), (↓ P x) tr.
-Proof. rewrite /trace_now /pred_at. intros H. by destruct tr. Qed.
-
-Lemma trace_andI {S L} (P Q : trace S L → Prop) (tr : trace S L) :
-  trace_and P Q tr ↔ P tr ∧ Q tr.
-Proof. Admitted.
-
-Lemma trace_nextI {S L} (P : trace S L → Prop) s l (tr : trace S L) :
-  P tr → (○ P) (s -[l]-> tr).
-Proof. intros ???. simpl in *. by simplify_eq. Qed.
 
 Lemma deliver_next_buffer msg mtr :
   mtrace_valid mtr →
